<?xml version="1.0"?>
<rdf:RDF xmlns="http://w3id.org/rec/Core/"
     xml:base="http://w3id.org/rec/Core/"
     xmlns:rdf="http://www.w3.org/1999/02/22-rdf-syntax-ns#"
     xmlns:owl="http://www.w3.org/2002/07/owl#"
     xmlns:xml="http://www.w3.org/XML/1998/namespace"
     xmlns:xsd="http://www.w3.org/2001/XMLSchema#"
     xmlns:rdfs="http://www.w3.org/2000/01/rdf-schema#"
     xmlns:Core="http://w3id.org/rec/Core/">
    <owl:Ontology rdf:about="http://w3id.org/rec/Core/">
        <owl:versionIRI rdf:resource="http://w3id.org/rec/Core/2.1/"/>
    </owl:Ontology>
    


    <!-- 
    ///////////////////////////////////////////////////////////////////////////////////////
    //
    // Annotation properties
    //
    ///////////////////////////////////////////////////////////////////////////////////////
     -->

    


    <!-- http://w3id.org/rec/Core/Example -->

    <owl:AnnotationProperty rdf:about="http://w3id.org/rec/Core/Example"/>
    


    <!-- http://w3id.org/rec/Core/IPSOComparable -->

    <owl:AnnotationProperty rdf:about="http://w3id.org/rec/Core/IPSOComparable"/>
    


    <!-- 
    ///////////////////////////////////////////////////////////////////////////////////////
    //
    // Object Properties
    //
    ///////////////////////////////////////////////////////////////////////////////////////
     -->

    


    <!-- http://w3id.org/rec/Core/hasBearing -->

    <owl:ObjectProperty rdf:about="http://w3id.org/rec/Core/hasBearing">
        <rdfs:domain rdf:resource="http://w3id.org/rec/Core/GeoReferenceOrigo"/>
        <rdfs:comment xml:lang="en">The angle between one of the axis of a local coordinate system within e.g. a building and a north-south meridian. The angle is measured between the meridian and the local coordinate axis and counted as positive to the east side of the meridan (neagtive to the west side).

Bearings are never greater than 90°.
Bearings are based on true north.</rdfs:comment>
    </owl:ObjectProperty>
    


    <!-- http://w3id.org/rec/Core/hasGeoReferenceOrigo -->

    <owl:ObjectProperty rdf:about="http://w3id.org/rec/Core/hasGeoReferenceOrigo">
        <rdfs:domain rdf:resource="http://w3id.org/rec/Core/Location"/>
    </owl:ObjectProperty>
    


    <!-- http://w3id.org/rec/Core/isLocatedAt -->

    <owl:ObjectProperty rdf:about="http://w3id.org/rec/Core/isLocatedAt">
        <rdfs:range rdf:resource="http://w3id.org/rec/Core/Location"/>
        <rdfs:comment xml:lang="se">Ett objekt som är av en klass som har en Location uttrycker detta med [myObject] locatedAt [myLocation].

Jämför: Ett objekt kan beskriva sin plats genom [myObject] locatedIn [myOtherObject], där annatObject är ett rum, en byggnad eller annan klass som har en plats (Location).</rdfs:comment>
    </owl:ObjectProperty>
    


    <!-- http://w3id.org/rec/Core/isLocatedIn -->

    <owl:ObjectProperty rdf:about="http://w3id.org/rec/Core/isLocatedIn">
        <rdfs:comment xml:lang="se">Ett objekt kan beskriva sin plats genom [myObject] locatedIn [myOtherObject], där annatObject är ett rum, en byggnad eller annan klass som har en plats (Location).

Jämför:Ett objekt som är av en klass som har en Location uttrycker detta med [myObject] locatedAt [myLocation].</rdfs:comment>
    </owl:ObjectProperty>
    


    <!-- 
    ///////////////////////////////////////////////////////////////////////////////////////
    //
    // Classes
    //
    ///////////////////////////////////////////////////////////////////////////////////////
     -->

    


    <!-- http://w3id.org/rec/Core/Agent -->

    <owl:Class rdf:about="http://w3id.org/rec/Core/Agent"/>
    


    <!-- http://w3id.org/rec/Core/GeoReferenceOrigo -->

    <owl:Class rdf:about="http://w3id.org/rec/Core/GeoReferenceOrigo">
        <rdfs:comment xml:lang="en">A fixed point for e.g. a building structure. Commonly refered to as &quot;insertion point&quot; in CAD-programs. Used as origo for LocalLocation.</rdfs:comment>
    </owl:Class>
    


    <!-- http://w3id.org/rec/Core/Id -->

    <owl:Class rdf:about="http://w3id.org/rec/Core/Id">
        <rdfs:comment xml:lang="en">An universally unique identifier (UUID) is a 128-bit number used to identify information in computer systems. Version 4 is prefered (random generated).</rdfs:comment>
    </owl:Class>
    


    <!-- http://w3id.org/rec/Core/Location -->

    <owl:Class rdf:about="http://w3id.org/rec/Core/Location">
        <Example xml:lang="en">59.33755390;18.05568540;32.500</Example>
        <IPSOComparable xml:lang="en">Altitude: 3321
Location: 3336
Latitude: 5513
Longitude: 5514 
Altitude: 5515</IPSOComparable>
        <rdfs:comment xml:lang="se">Placeringen av ett objekt (exempelvis sensor eller objekt) eller position för objekt i ett geografiskt kartsystem eller inom omslutningen av ett annat objekt. Vi använder WGS84. Formatet är i decimalgrader (DD).</rdfs:comment>
        <rdfs:comment xml:lang="en">The absolute location of a point (expressed in WGS84).</rdfs:comment>
    </owl:Class>
    


    <!-- http://w3id.org/rec/Core/MeasurementUnit -->

    <owl:Class rdf:about="http://w3id.org/rec/Core/MeasurementUnit"/>
    


    <!-- http://w3id.org/rec/Core/Name -->

    <owl:Class rdf:about="http://w3id.org/rec/Core/Name">
        <rdfs:comment xml:lang="en">Human-friendly name.</rdfs:comment>
    </owl:Class>
    


    <!-- http://w3id.org/rec/Core/ObservationDuration -->

    <owl:Class rdf:about="http://w3id.org/rec/Core/ObservationDuration">
        <rdfs:subClassOf rdf:resource="http://w3id.org/rec/Core/Time"/>
        <rdfs:comment xml:lang="en">Length of observation in ms.</rdfs:comment>
    </owl:Class>
    


    <!-- http://w3id.org/rec/Core/ObservationTime -->

    <owl:Class rdf:about="http://w3id.org/rec/Core/ObservationTime">
        <rdfs:subClassOf rdf:resource="http://w3id.org/rec/Core/Time"/>
        <rdfs:comment xml:lang="en">Time for made observation.</rdfs:comment>
    </owl:Class>
    


    <!-- http://w3id.org/rec/Core/ProcessedTime -->

    <owl:Class rdf:about="http://w3id.org/rec/Core/ProcessedTime">
        <rdfs:subClassOf rdf:resource="http://w3id.org/rec/Core/Time"/>
        <rdfs:comment xml:lang="en">Time when an object or result was processed in a system.</rdfs:comment>
    </owl:Class>
    


    <!-- http://w3id.org/rec/Core/SourceData -->

    <owl:Class rdf:about="http://w3id.org/rec/Core/SourceData"/>
    


    <!-- http://w3id.org/rec/Core/StartTime -->

    <owl:Class rdf:about="http://w3id.org/rec/Core/StartTime">
        <rdfs:subClassOf rdf:resource="http://w3id.org/rec/Core/Time"/>
        <rdfs:comment xml:lang="en">Start time.</rdfs:comment>
    </owl:Class>
    


    <!-- http://w3id.org/rec/Core/StopTime -->

    <owl:Class rdf:about="http://w3id.org/rec/Core/StopTime">
        <rdfs:subClassOf rdf:resource="http://w3id.org/rec/Core/Time"/>
        <rdfs:comment xml:lang="en">Stop time.</rdfs:comment>
    </owl:Class>
    


    <!-- http://w3id.org/rec/Core/Time -->

    <owl:Class rdf:about="http://w3id.org/rec/Core/Time">
        <rdfs:comment xml:lang="se">Tidsdomänen innehåller klasser som beskriver start- och stopptid, duration mm.

Tidsformat:

ISO8601

Komplett datum plus timmar, mintuer, sekunder och decimal del av sekund.

      YYYY-MM-DDThh:mm:ss.sTZD (eg 1997-07-16T19:20:30.45+01:00)

Där:

     YYYY = 4 siffror för år.
     MM   = 2 siffror månad (01=januari, etc.)
     DD   = 2 siffror för dag i månad (01 till 31)
     hh   = 2 siffror för timme (00 till 23) (am/pm INTE tillåtet)
     mm   = 2 siffror för minuter (00 till 59)
     ss   = 2 siffror för sekund (00 till 59)
     s    =  1 eller flera siffror representerar en decimal fraktion av en sekund

     TZD  = time zone designator (Z eller +hh:mm eller -hh:mm)

Tid är uttryckt i UTC (Coordinated Universal Time), med speciell UTC anvisare (&quot;Z&quot;) för GMT.</rdfs:comment>
    </owl:Class>
    


    <!-- 
    ///////////////////////////////////////////////////////////////////////////////////////
    //
    // Individuals
    //
    ///////////////////////////////////////////////////////////////////////////////////////
     -->

    


    <!-- http://w3id.org/rec/Core/A -->

    <owl:NamedIndividual rdf:about="http://w3id.org/rec/Core/A">
        <rdf:type rdf:resource="http://w3id.org/rec/Core/MeasurementUnit"/>
        <rdfs:comment xml:lang="en">Ampere. Current in a circuit.</rdfs:comment>
    </owl:NamedIndividual>
    


    <!-- http://w3id.org/rec/Core/C -->

    <owl:NamedIndividual rdf:about="http://w3id.org/rec/Core/C">
        <rdf:type rdf:resource="http://w3id.org/rec/Core/MeasurementUnit"/>
        <rdfs:comment xml:lang="en">Temperature in Celsius degress. Note that correct SI Unit is Kelvin.</rdfs:comment>
    </owl:NamedIndividual>
    


    <!-- http://w3id.org/rec/Core/F -->

    <owl:NamedIndividual rdf:about="http://w3id.org/rec/Core/F">
        <rdf:type rdf:resource="http://w3id.org/rec/Core/MeasurementUnit"/>
        <rdfs:comment xml:lang="en">Temperature in Fahrenheit degress.</rdfs:comment>
    </owl:NamedIndividual>
    


    <!-- http://w3id.org/rec/Core/Hz -->

    <owl:NamedIndividual rdf:about="http://w3id.org/rec/Core/Hz">
        <rdf:type rdf:resource="http://w3id.org/rec/Core/MeasurementUnit"/>
        <rdfs:comment xml:lang="en">One cycle per second.</rdfs:comment>
    </owl:NamedIndividual>
    


    <!-- http://w3id.org/rec/Core/K -->

    <owl:NamedIndividual rdf:about="http://w3id.org/rec/Core/K">
        <rdf:type rdf:resource="http://w3id.org/rec/Core/MeasurementUnit"/>
        <rdfs:comment xml:lang="en">Temperature in Kelvin degrees</rdfs:comment>
    </owl:NamedIndividual>
    


    <!-- http://w3id.org/rec/Core/Pa -->

    <owl:NamedIndividual rdf:about="http://w3id.org/rec/Core/Pa">
        <rdf:type rdf:resource="http://w3id.org/rec/Core/MeasurementUnit"/>
        <rdfs:comment xml:lang="en">The pascal is the SI derived unit of pressure used to quantify internal pressure, stress. It is defined as one newton per square metre.</rdfs:comment>
    </owl:NamedIndividual>
    


    <!-- http://w3id.org/rec/Core/Pf -->

    <owl:NamedIndividual rdf:about="http://w3id.org/rec/Core/Pf">
        <rdf:type rdf:resource="http://w3id.org/rec/Core/MeasurementUnit"/>
        <rdfs:comment xml:lang="en">The power factor of an AC electrical power system is defined as the ratio of the real power flowing to the load to the apparent power in the circuit, and is a dimensionless number in the closed interval of −1 to 1.</rdfs:comment>
    </owl:NamedIndividual>
    


    <!-- http://w3id.org/rec/Core/RH -->

    <owl:NamedIndividual rdf:about="http://w3id.org/rec/Core/RH">
        <rdf:type rdf:resource="http://w3id.org/rec/Core/MeasurementUnit"/>
        <rdfs:comment xml:lang="en">Relative Humidity. The amount of water vapour present in air expressed as a percentage of the amount needed for saturation at the same temperature.</rdfs:comment>
    </owl:NamedIndividual>
    


    <!-- http://w3id.org/rec/Core/V -->

    <owl:NamedIndividual rdf:about="http://w3id.org/rec/Core/V">
        <rdf:type rdf:resource="http://w3id.org/rec/Core/MeasurementUnit"/>
        <rdfs:comment xml:lang="en">Voltage, electric potential difference, is the difference in electric potential between two points.</rdfs:comment>
    </owl:NamedIndividual>
    


    <!-- http://w3id.org/rec/Core/W -->

    <owl:NamedIndividual rdf:about="http://w3id.org/rec/Core/W">
        <rdf:type rdf:resource="http://w3id.org/rec/Core/MeasurementUnit"/>
        <rdfs:comment xml:lang="en">This unit is typically used to express the momentaneous output power of engines and the power of electric motors, tools, machines, and heaters.</rdfs:comment>
    </owl:NamedIndividual>
    


    <!-- http://w3id.org/rec/Core/Wh -->

    <owl:NamedIndividual rdf:about="http://w3id.org/rec/Core/Wh">
        <rdf:type rdf:resource="http://w3id.org/rec/Core/MeasurementUnit"/>
        <rdfs:comment xml:lang="en">Enery. Watthour.</rdfs:comment>
    </owl:NamedIndividual>
    


    <!-- http://w3id.org/rec/Core/kg -->

    <owl:NamedIndividual rdf:about="http://w3id.org/rec/Core/kg">
        <rdf:type rdf:resource="http://w3id.org/rec/Core/MeasurementUnit"/>
        <rdfs:comment xml:lang="en">Mass.</rdfs:comment>
    </owl:NamedIndividual>
    


    <!-- http://w3id.org/rec/Core/m -->

    <owl:NamedIndividual rdf:about="http://w3id.org/rec/Core/m">
        <rdf:type rdf:resource="http://w3id.org/rec/Core/MeasurementUnit"/>
        <rdfs:comment xml:lang="en">Lenght.</rdfs:comment>
    </owl:NamedIndividual>
    


    <!-- http://w3id.org/rec/Core/m2 -->

    <owl:NamedIndividual rdf:about="http://w3id.org/rec/Core/m2">
        <rdf:type rdf:resource="http://w3id.org/rec/Core/MeasurementUnit"/>
        <rdfs:comment xml:lang="en">Area unit. It is the area of a square whose sides measure exactly one metre.</rdfs:comment>
    </owl:NamedIndividual>
    


    <!-- http://w3id.org/rec/Core/m3 -->

    <owl:NamedIndividual rdf:about="http://w3id.org/rec/Core/m3">
        <rdf:type rdf:resource="http://w3id.org/rec/Core/MeasurementUnit"/>
        <rdfs:comment xml:lang="en">Volume is the quantity of three-dimensional space enclosed by a closed surface, for example, the space that a substance (solid, liquid, gas, or plasma) or shape occupies or contains. Volume is often quantified numerically using the cubic metre (m3).</rdfs:comment>
    </owl:NamedIndividual>
    


    <!-- http://w3id.org/rec/Core/s -->

    <owl:NamedIndividual rdf:about="http://w3id.org/rec/Core/s">
        <rdf:type rdf:resource="http://w3id.org/rec/Core/MeasurementUnit"/>
        <rdfs:comment xml:lang="en">The second is the duration of 9 192 631 770 periods of the radiation corresponding to the transition between the two hyperfine levels of the ground state of the cesium 133 atom.</rdfs:comment>
    </owl:NamedIndividual>
</rdf:RDF>



<!-- Generated by the OWL API (version 4.2.8.20170104-2310) https://github.com/owlcs/owlapi -->

