<?xml version="1.0"?>
<rdf:RDF
    xmlns:rdf="http://www.w3.org/1999/02/22-rdf-syntax-ns#"
    xmlns:core="https://w3id.org/rec/core/"
    xmlns="https://w3id.org/rec/agents/"
    xmlns:rdfs="http://www.w3.org/2000/01/rdf-schema#"
    xmlns:dcterms="http://purl.org/dc/terms/"
    xmlns:dc="http://purl.org/dc/elements/1.1/"
    xmlns:owl="http://www.w3.org/2002/07/owl#"
    xmlns:o2o="https://karlhammar.com/owl2oas/o2o.owl#"
    xmlns:skos="http://www.w3.org/2004/02/skos/core#"
    xmlns:cc="http://creativecommons.org/ns#"
    xmlns:vann="http://purl.org/vocab/vann/"
    xmlns:cpannotationschema="http://www.ontologydesignpatterns.org/schemas/cpannotationschema.owl#"
    xmlns:xsd="http://www.w3.org/2001/XMLSchema#"
  xml:base="https://w3id.org/rec/agents/">
  <owl:Ontology rdf:about="">
    <vann:preferredNamespaceUri>https://w3id.org/rec/agents/3.1.1/</vann:preferredNamespaceUri>
    <rdfs:comment xml:lang="en">The Agents module is work-in-progress; requirements are rather unclear as of yet.</rdfs:comment>
    <owl:versionIRI rdf:resource="https://w3id.org/rec/agents/3.1.1/"/>
    <owl:imports rdf:resource="https://w3id.org/rec/core/3.1.1/"/>
    <dc:title>RealEstateCore Agents Module</dc:title>
    <cpannotationschema:coversRequirements xml:lang="en">What is Karl Hammar's GitHub account ID?</cpannotationschema:coversRequirements>
    <owl:versionInfo>3.1.1</owl:versionInfo>
    <rdfs:seeAlso rdf:resource="https://w3id.org/rec/"/>
    <dc:publisher>RealEstateCore Consortium</dc:publisher>
    <dc:creator>Karl Hammar</dc:creator>
    <dcterms:modified>2020-04-21</dcterms:modified>
    <cpannotationschema:coversRequirements xml:lang="en">What is the RealEstateCore organizational GitHub account ID?</cpannotationschema:coversRequirements>
    <cc:license rdf:resource="https://opensource.org/licenses/MIT"/>
    <vann:preferredNamespacePrefix>agents</vann:preferredNamespacePrefix>
    <dc:description xml:lang="en">This REC model covers basic types of agents (people, organizations, groups), structurally mostly aligned with FOAF -- divergences are noted in the respective propertys' documentation.</dc:description>
    <cpannotationschema:coversRequirements xml:lang="en">Who are the members of the RealEstateCore release engineering team?</cpannotationschema:coversRequirements>
  </owl:Ontology>
  <owl:Class rdf:about="https://w3id.org/rec/agents/Group">
    <rdfs:seeAlso rdf:resource="http://xmlns.com/foaf/0.1/Group"/>
    <rdfs:label xml:lang="en">Group</rdfs:label>
    <rdfs:comment xml:lang="en">A collection of individual Agents (included in the Group via the object property hasMember).</rdfs:comment>
    <rdfs:subClassOf rdf:resource="https://w3id.org/rec/core/Agent"/>
  </owl:Class>
  <owl:Class rdf:about="https://w3id.org/rec/agents/Organization">
    <rdfs:seeAlso rdf:resource="http://xmlns.com/foaf/0.1/Organization"/>
    <rdfs:label xml:lang="en">Organization</rdfs:label>
    <rdfs:comment xml:lang="en">An organization of any sort (e.g., a business, association, project, consortium, tribe, etc.)</rdfs:comment>
    <rdfs:subClassOf rdf:resource="https://w3id.org/rec/core/Agent"/>
  </owl:Class>
  <owl:Class rdf:about="https://w3id.org/rec/agents/Person">
    <rdfs:seeAlso rdf:resource="http://xmlns.com/foaf/0.1/Person"/>
    <rdfs:label xml:lang="en">Person</rdfs:label>
    <rdfs:comment xml:lang="en">A natural person (i.e., an individual human being).</rdfs:comment>
    <rdfs:subClassOf rdf:resource="https://w3id.org/rec/core/Agent"/>
  </owl:Class>
  <owl:ObjectProperty rdf:about="https://w3id.org/rec/agents/account">
    <rdfs:seeAlso rdf:resource="http://xmlns.com/foaf/0.1/account"/>
    <rdfs:label xml:lang="en">account</rdfs:label>
    <rdfs:comment xml:lang="en">An online account that an Agent holds.</rdfs:comment>
    <rdfs:domain rdf:resource="https://w3id.org/rec/core/Agent"/>
  </owl:ObjectProperty>
  <owl:ObjectProperty rdf:about="https://w3id.org/rec/agents/hasMember">
    <rdfs:seeAlso rdf:resource="http://xmlns.com/foaf/0.1/member"/>
    <rdfs:label xml:lang="en">has member</rdfs:label>
    <rdfs:comment xml:lang="en">Indicates the member Agents that are part of a certain Group.</rdfs:comment>
    <rdfs:range rdf:resource="https://w3id.org/rec/core/Agent"/>
    <rdfs:domain rdf:resource="https://w3id.org/rec/agents/Group"/>
  </owl:ObjectProperty>
  <owl:ObjectProperty rdf:about="https://w3id.org/rec/agents/logo">
    <rdfs:seeAlso rdf:resource="http://xmlns.com/foaf/0.1/logo"/>
    <rdfs:label xml:lang="en">logo</rdfs:label>
    <rdfs:comment xml:lang="en">Links an Organization to an image/logo that represents them. This is stricter than FOAF, in which logo has domain "Thing"; but it works for our domain.</rdfs:comment>
    <rdfs:domain rdf:resource="https://w3id.org/rec/agents/Organization"/>
  </owl:ObjectProperty>
  <owl:ObjectProperty rdf:about="https://w3id.org/rec/agents/image">
    <rdfs:seeAlso rdf:resource="http://xmlns.com/foaf/0.1/img"/>
    <rdfs:label xml:lang="en">image</rdfs:label>
    <rdfs:comment xml:lang="en">Property that links a Person to an image that represents them.</rdfs:comment>
    <rdfs:domain rdf:resource="https://w3id.org/rec/agents/Person"/>
  </owl:ObjectProperty>
  <owl:DatatypeProperty rdf:about="https://w3id.org/rec/agents/name">
    <rdfs:label xml:lang="en">name</rdfs:label>
    <rdfs:comment xml:lang="en">A name for some Agent. Stricter than FOAF, we assume that things that have names are Agents, not Things (e.g., other predicates will need be used to described identifiers for non-Agents).</rdfs:comment>
    <rdfs:comment rdf:resource="http://xmlns.com/foaf/0.1/name"/>
    <rdfs:domain rdf:resource="https://w3id.org/rec/core/Agent"/>
  </owl:DatatypeProperty>
  <owl:DatatypeProperty rdf:about="https://w3id.org/rec/agents/familyName">
    <rdfs:seeAlso rdf:resource="http://xmlns.com/foaf/0.1/familyName"/>
    <rdfs:label xml:lang="en">family name</rdfs:label>
    <rdfs:comment xml:lang="en">A person's family name.</rdfs:comment>
    <rdfs:domain rdf:resource="https://w3id.org/rec/agents/Person"/>
    <rdfs:subPropertyOf rdf:resource="https://w3id.org/rec/agents/name"/>
  </owl:DatatypeProperty>
  <owl:DatatypeProperty rdf:about="https://w3id.org/rec/agents/lastName">
    <rdfs:label xml:lang="en">last name</rdfs:label>
    <rdfs:comment xml:lang="en">A person's last name (if they have one; this varies across cultural contexts).</rdfs:comment>
    <rdfs:comment rdf:resource="http://xmlns.com/foaf/0.1/lastName"/>
    <rdfs:domain rdf:resource="https://w3id.org/rec/agents/Person"/>
    <rdfs:subPropertyOf rdf:resource="https://w3id.org/rec/agents/name"/>
  </owl:DatatypeProperty>
  <owl:DatatypeProperty rdf:about="https://w3id.org/rec/agents/firstName">
    <rdfs:seeAlso rdf:resource="http://xmlns.com/foaf/0.1/firstName"/>
    <rdfs:label xml:lang="en">first name</rdfs:label>
    <rdfs:comment xml:lang="en">A person's first name (if they have one; this varies across cultural contexts).</rdfs:comment>
    <rdfs:domain rdf:resource="https://w3id.org/rec/agents/Person"/>
    <rdfs:subPropertyOf rdf:resource="https://w3id.org/rec/agents/name"/>
  </owl:DatatypeProperty>
  <owl:DatatypeProperty rdf:about="https://w3id.org/rec/agents/givenName">
    <rdfs:seeAlso rdf:resource="http://xmlns.com/foaf/0.1/givenName"/>
    <rdfs:label xml:lang="en">given name</rdfs:label>
    <rdfs:comment xml:lang="en">A person's personal, individual name.</rdfs:comment>
    <rdfs:domain rdf:resource="https://w3id.org/rec/agents/Person"/>
    <rdfs:subPropertyOf rdf:resource="https://w3id.org/rec/agents/name"/>
  </owl:DatatypeProperty>
  <owl:FunctionalProperty rdf:about="https://w3id.org/rec/agents/gender">
    <rdfs:seeAlso rdf:resource="http://xmlns.com/foaf/0.1/gender"/>
    <rdfs:label xml:lang="en">gender</rdfs:label>
    <rdfs:comment xml:lang="en">A gender designation for a Person. Stricter than FOAF, which allows all Agents to have gender.</rdfs:comment>
    <rdfs:domain rdf:resource="https://w3id.org/rec/agents/Person"/>
    <rdf:type rdf:resource="http://www.w3.org/2002/07/owl#DatatypeProperty"/>
  </owl:FunctionalProperty>
</rdf:RDF>

<!-- Created with TopBraid -->
